\begin{gather*}
    P_{si}^{\sigma_s} = P_s^{\sigma_s} Y_s Y_{si}^{-1} 
    \Rightarrow (P_{si}Y_{si})^{\sigma_s} = P_s^{\sigma_s} Y_s Y_{si}^{\sigma_s-1}
    \Rightarrow (P_{si}Y_{si})^{\sigma_s} = (P_sY_s)(P_sY_{si})^{\sigma_s-1}\\
    \Rightarrow (P_{si}Y_{si})^{\frac{\sigma_s}{\sigma_s-1}} = (P_sY_s)^{\frac{1}{\sigma_s-1}}P_sY_{si}\\
    \Rightarrow Y_{si} = \dfrac{(P_{si}Y_{si})^{\frac{\sigma_s}{\sigma_s-1}}}{P_s(P_sY_s)^{\frac{1}{\sigma_s-1}}}\\
    \Rightarrow \hat{A}_{si} = \frac{1}{P_s(P_sY_s)^{\frac{1}{\sigma_s-1}}}\dfrac{(P_{si}Y_{si})^{\frac{\sigma_s}{\sigma_s-1}}}{\hat{K}_{si}^{\beta_s} L_{si}^{1-\beta_s}} = \input{model_elements/production technology compress.tex}
\end{gather*}